

Supplements: Differentially Private Selection using Smooth Sensitivity

This provides the omitted proofs in the main paper.

I. PROOFS

A. Theorem 3

Theorem 3. If Z_r are derived from g , the smooth private selection mechanism satisfies ~~$\left(\left(k + \frac{|\mathcal{R}|-1}{2} \cdot l\right) \cdot \epsilon\right)$~~ $\left(\left(k + \frac{|\mathcal{R}|}{2} \cdot l\right) \cdot \epsilon\right)$ -differential privacy.

Proof. The following proof is wrong. The correct proof is similar to that of Theorem 2. However, actually, the mechanism's differential privacy guarantee should be less than $\left(\left(k + \frac{|\mathcal{R}|-1}{2} \cdot l\right) \cdot \epsilon\right)$ when using an appropriate (α, β) -admissible distribution. In our next paper, this point will be discussed in detail.

We let $\mathcal{R} = \{1, 2, \dots, m\}$ as in the proof of Theorem 2. It is sufficient to show that, for all neighboring datasets $x, y \in D^n$,

$$\begin{aligned} & \Pr[M(x) = 1] \\ & \leq \exp\left(\left(k + \frac{m-1}{2} \cdot l\right) \cdot \epsilon\right) \cdot \Pr[M(y) = 1]. \end{aligned} \quad (1)$$

Here, the relations

$$\begin{aligned} \Pr[M(x) = 1] &= \int_{v \in (-\infty, \infty)} \Pr\left[Z_1 = \frac{\alpha'(v - u(x, 1))}{S(x)}\right] \\ &\quad \cdot \Pr\left[Z_2 \leq \frac{\alpha'(v - u(x, 2))}{S(x)}\right] \\ &\quad \cdots \Pr\left[Z_m \leq \frac{\alpha'(v - u(x, m))}{S(x)}\right] \end{aligned} \quad (2)$$

and

$$\begin{aligned} & \Pr[M(y) = 1] \\ & \geq \int_{v \in (-\infty, \infty)} \Pr\left[Z_1 = \frac{\alpha'(v - u(y, 1) + S(x))}{S(y)}\right] \\ &\quad \cdot \Pr\left[Z_2 \leq \frac{\alpha'(v - u(x, 2))}{S(y)}\right] \\ &\quad \cdots \Pr\left[Z_m \leq \frac{\alpha'(v - u(x, m))}{S(y)}\right] \end{aligned} \quad (3)$$

hold as in the proof of Theorem 2, and in particular, we should note $u(x, 1) - u(y, 1) + S(x) \geq 0$.

(I) When $S(x) \geq S(y)$:

Because $\forall r \in \{2, 3, \dots, m\}$:

$$\Pr\left[Z_r \leq \frac{\alpha'(v - u(x, r))}{S(y)}\right] \geq \Pr\left[Z_r \leq \frac{\alpha'(v - u(x, r))}{S(x)}\right],$$

[\because the property of g]

$$\begin{aligned} (3) & \geq \int_{v \in (-\infty, \infty)} \Pr\left[Z_1 = \frac{\alpha'(v - u(y, 1) + S(x))}{S(y)}\right] \\ &\quad \cdot \Pr\left[Z_2 \leq \frac{\alpha'(v - u(x, 2))}{S(x)}\right] \\ &\quad \cdots \Pr\left[Z_m \leq \frac{\alpha'(v - u(x, m))}{S(x)}\right]. \end{aligned} \quad (4)$$

From (2) and (4), the following relation holds:

$$\Pr[M(x) = 1] \leq \exp\left(\left(k + \frac{l}{2}\right) \cdot \epsilon\right) \cdot \Pr[M(y) = 1].$$

(II) When $S(x) < S(y)$:

Because

$$\begin{aligned} & \Pr\left[Z_1 = \frac{\alpha'(v - u(y, 1) + S(x))}{S(y)}\right] \\ & \geq \Pr\left[Z_1 = \frac{\alpha'(v - u(y, 1) + S(x))}{S(x)}\right], \end{aligned}$$

[\because the property of g]

\leftarrow This is wrong.

$$\begin{aligned} (3) & \geq \int_{v \in (-\infty, \infty)} \Pr\left[Z_1 = \frac{\alpha'(v - u(y, 1) + S(x))}{S(x)}\right] \\ &\quad \cdot \Pr\left[Z_2 \leq \frac{\alpha'(v - u(x, 2))}{S(y)}\right] \\ &\quad \cdots \Pr\left[Z_m \leq \frac{\alpha'(v - u(x, m))}{S(y)}\right]. \end{aligned} \quad (5)$$

From (2) and (5), the relation (1) holds. \square

B. Theorem 5

Theorem 5. Given a threshold T , we let the set of x satisfying $LS_f(x) > T$ be U . For any $\beta (> 0)$ satisfying

$$\beta \leq \min_{x \notin U} \frac{1}{ud(x)} \cdot \ln\left(\frac{GS_f}{LS_f(x)}\right), \quad (6)$$

where $ud(x) := \min_{y \in U} d(y, x)$ represents the shortest distance between x and U , the following function S is a β -smooth upper bound:

$$S(x) = GS_f \cdot e^{-\beta \cdot ud(x)}.$$

Proof. From (6), for all $x \notin U$,

$$\beta \leq \frac{1}{ud(x)} \cdot \ln \left(\frac{GS_f}{LS_f(x)} \right) \\ \iff LS_f(x) \leq GS_f \cdot e^{-\beta \cdot ud(x)}.$$

Therefore, from Definition 4 (for β -smooth upper bound), it is sufficient to show that

$$\forall x, y, d(x, y) = 1 : S(x) \leq e^\beta \cdot S(y). \quad (7)$$

(I) When $x, y \in U$:

Because $S(x) = S(y) = GS_f$, the relation (7) holds.

(II) When $x \in U$ and $y \notin U$:

Because $S(x) = GS_f$ and

$$S(y) = GS_f \cdot e^{-\beta}, \quad [\cdot : ud(y) = d(x, y) = 1]$$

the relation (7) holds.

(III) When $x \notin U$ and $y \in U$:

Similar to Case (II), $S(x) = GS_f \cdot e^{-\beta}$ and $S(y) = GS_f$; therefore, the relation (7) holds.

(IV) When $x, y \notin U$:

Where X satisfies $X \in U$ and $d(X, x) = ud(x)$, and Y satisfies $Y \in U$ and $d(Y, y) = ud(y)$,

$$\begin{aligned} e^\beta \cdot S(y) &= e^\beta \cdot GS_f \cdot e^{-\beta \cdot d(Y, y)} \\ &\geq e^\beta \cdot GS_f \cdot e^{-\beta \cdot d(X, y)} \quad [\cdot : d(Y, y) \leq d(X, y)] \\ &\geq e^\beta \cdot GS_f \cdot e^{-\beta \cdot (d(X, x) + d(x, y))} \\ &\quad [\cdot : d(X, y) \leq d(X, x) + d(x, y)] \\ &= GS_f \cdot e^{-\beta \cdot d(X, x)} = S(x). \quad [\cdot : d(x, y) = 1] \end{aligned}$$

Therefore, the relation (7) holds. \square

C. Lemma 2

Lemma 2. (b, c) satisfies $LS_{\chi_{TDT}^2}((b, c)) > 6$ when

$$\begin{aligned} 0 \leq c < \frac{b-8}{7} \vee 2 \leq b < \frac{c+8}{7} \\ \vee \quad 0 \leq b < \frac{c-8}{7} \vee 2 \leq c < \frac{b+8}{7}. \end{aligned}$$

Proof. $LS_{\chi_{TDT}^2}(x) > 6$ can be satisfied only if $x = (b, c)$ and $y = (b-2, c+2) \vee (b+2, c-2)$.

When $y = (b-2, c+2)$ is possible, $b \geq 2$ and $c \geq 0$. In this case,

$$\begin{aligned} &\chi_{TDT}^2(b, c) - \chi_{TDT}^2(b-2, c+2) \\ &= \frac{(b-c)^2}{b+c} - \frac{(b-c-4)^2}{b+c} = \frac{8(b-c-2)}{b+c}. \quad (8) \end{aligned}$$

$|8| > 6 \iff c < \frac{b-8}{7} \vee b < \frac{c+8}{7}$; therefore, (b, c) satisfies $LS_{\chi_{TDT}^2}((b, c)) > 6$ when $0 \leq c < \frac{b-8}{7} \vee 2 \leq b < \frac{c+8}{7}$.

Similarly when $y = (b+2, c-2)$ is possible, we can obtain $0 \leq b < \frac{c-8}{7} \vee 2 \leq c < \frac{b+8}{7}$. \square

D. Lemma 3

Lemma 3. The Hamming distance for TDT datasets can be

$$\begin{aligned} &d(T(b, c), T(b', c')) \\ &= \begin{cases} \left\lceil \frac{|(b+c)-(b'+c')|}{2} \right\rceil & ((b-b') \cdot (c-c') \geq 0) \\ \left\lceil \frac{\max\{|b-b'|, |c-c'|\}}{2} \right\rceil & ((b-b') \cdot (c-c') < 0) \end{cases}, \end{aligned}$$

where $T(b, c)$ represents a table that can be formed as the following table:

		Non-Transmitted Allele		Total
		A_1	A_2	
Transmitted Allele	A_1	a	b	$a+b$
	A_2	c	d	$c+d$
Total		$a+c$	$b+d$	$2N$

Proof. The possible changes in (b, c) between neighboring datasets are

(b, c)

$$\begin{aligned} \rightarrow & (b-2, c), (b-2, c+1), (b-2, c+2), \\ & (b-1, c-1), (b-1, c), (b-1, c+1), (b-1, c+2), \\ & (b, c-2), (b, c-1), (b, c), (b, c+1), (b, c+2), \\ & (b+1, c-2), (b+1, c-1), (b+1, c), (b+1, c+1), \\ & (b+2, c-2), (b+2, c-1), (b+2, c). \end{aligned}$$

Therefore, the maximum change in the value of $b+c$ is 2; when $(b-b') \cdot (c-c') \geq 0$, the Hamming distance can be

$$d(T(b, c), T(b', c')) = \left\lceil \frac{|(b+c)-(b'+c')|}{2} \right\rceil.$$

When $(b-b') \cdot (c-c') < 0$, using the changes $(b, c) \rightarrow (b-2, c), (b-2, c+1), (b-2, c+2), (b+2, c-2), (b+2, c-1), (b+2, c)$, the Hamming distance can be

$$d(T(b, c), T(b', c')) = \left\lceil \frac{\max\{|b-b'|, |c-c'|\}}{2} \right\rceil. \quad \square$$